Still working on [Rule] templates

src/Ex/RuleTemplate.v
@@ -9,6 +9,27 @@ Set Implicit Arguments.
 Local Open Scope list.
 Local Open Scope fmap.
 
+(** TODO: use [None] when silent transactions are supported. *)
+Definition addSilentUpRq (orq: ORq Msg) (mrss : list IdxT): ORq Msg :=
+  orq +[upRq <- {| rqi_msg := {| msg_id := 0;
+                                 msg_type := false;
+                                 msg_value := O |};
+                   rqi_minds_rss := mrss;
+                   rqi_midx_rsb := 0 |}].
+
+Record Miv :=
+  { miv_id: IdxT;
+    miv_value: Value }.
+
+Definition rqMsg (miv: Miv) :=
+  {| msg_id := miv_id miv;
+     msg_type := MRq;
+     msg_value := miv_value miv |}.
+Definition rsMsg (miv: Miv) :=
+  {| msg_id := miv_id miv;
+     msg_type := MRs;
+     msg_value := miv_value miv |}.
+
 Section Template.
   Variable (dtr: DTree).
   Context `{oifc: OStateIfc}.
@@ -17,81 +38,88 @@ Section Template.
   (* Heads-up: [cidx] is not the index of itself, but of a child. *)
   Definition immDownRule (cidx: IdxT)
              (prec: OPrec)
-             (trs: OState -> Msg -> option (OState * Msg)): Rule :=
+             (trs: OState -> Msg -> OState * Miv): Rule :=
     rule[ridx]
     :requires (MsgsFrom [rqUpFrom cidx] /\ MsgIdsFrom [msgId] /\
                RqAccepting /\ UpLockFree /\ DownLockFree /\ prec)
     :transition
        (do (st --> (msg <-- getFirstMsg st.(msgs);
-                    nst <-- trs st.(ost) msg;
-                    return {{ fst nst, st.(orq), [(downTo cidx, snd nst)] }}))).
+                      nst ::= trs st.(ost) msg;
+                    return {{ fst nst, st.(orq),
+                              [(downTo cidx, rsMsg (snd nst))] }}))).
   
   Definition immUpRule (oidx: IdxT)
              (prec: OPrec)
-             (trs: OState -> Msg -> option (OState * Msg)): Rule :=
+             (trs: OState -> Msg -> OState * Miv): Rule :=
     rule[ridx]
     :requires (MsgsFrom [downTo oidx] /\ MsgIdsFrom [msgId] /\
                RqAccepting /\ DownLockFree /\ prec)
     :transition
        (do (st --> (msg <-- getFirstMsg st.(msgs);
-                      nst <-- trs st.(ost) msg;
-                      return {{ fst nst, st.(orq), [(rqUpFrom oidx, snd nst)] }}))).
+                      nst ::= trs st.(ost) msg;
+                    return {{ fst nst, st.(orq),
+                              [(rsUpFrom oidx, rsMsg (snd nst))] }}))).
 
   Definition rqUpUpRule (cidx oidx: IdxT)
-             (prec: OPrec)
-             (trs: OState -> Msg -> option Msg): Rule :=
+             (prec: OState -> list (Id Msg) -> Prop)
+             (trs: OState -> Msg -> Miv): Rule :=
     rule[ridx]
     :requires (MsgsFrom [rqUpFrom cidx] /\ MsgIdsFrom [msgId] /\
-               RqAccepting /\ UpLockFree /\ prec)
+               RqAccepting /\ UpLockFree /\
+               fun ost _ mins => prec ost mins)
     :transition
        (do (st --> (msg <-- getFirstMsg st.(msgs);
-                      out <-- trs st.(ost) msg;
-                      return {{ st.(ost),
-                                addRq st.(orq) upRq msg [downTo oidx] (downTo cidx),
-                                [(rqUpFrom oidx, out)] }}))).
+                      out ::= trs st.(ost) msg;
+                    return {{ st.(ost),
+                              addRq st.(orq) upRq msg [downTo oidx] (downTo cidx),
+                              [(rqUpFrom oidx, rqMsg out)] }}))).
 
   Definition rqUpUpRuleS (oidx: IdxT)
              (prec: OPrec)
-             (trs: OState -> option Msg): Rule :=
+             (trs: OState -> Miv): Rule :=
     rule[ridx]
     :requires (MsgsFrom nil /\ RqAccepting /\ UpLockFree /\ prec)
     :transition
-       (do (st --> (out <-- trs st.(ost);
+       (do (st --> (out ::= trs st.(ost);
                     return {{ st.(ost),
                               addSilentUpRq st.(orq) [downTo oidx],
-                              [(rqUpFrom oidx, out)] }}))).
+                              [(rqUpFrom oidx, rqMsg out)] }}))).
 
   (** * FIXME: need to know children indices from [trs] are sound. *)
   Definition rqUpDownRule (cidx oidx: IdxT)
-             (prec: OPrec)
-             (trs: OState -> Msg -> option (list IdxT * Msg)): Rule :=
+             (prec: OState -> list (Id Msg) -> Prop)
+             (trs: OState -> Msg -> list IdxT * Miv): Rule :=
     rule[ridx]
     :requires (MsgsFrom [rqUpFrom cidx] /\ MsgIdsFrom [msgId] /\
-               RqAccepting /\ UpLockFree /\ DownLockFree /\ prec)
+               RqAccepting /\ UpLockFree /\ DownLockFree /\
+               fun ost _ mins => prec ost mins)
     :transition
        (do (st -->
                (msg <-- getFirstMsg st.(msgs);
-                  nst <-- trs st.(ost) msg;
+                  nst ::= trs st.(ost) msg;
                 return {{ st.(ost),
                           addRq st.(orq) downRq msg
                                          (map rsUpFrom (fst nst)) (downTo cidx),
-                          map (fun cidx => (downTo cidx, snd nst)) (fst nst) }}))).
+                          map (fun cidx => (downTo cidx, rqMsg (snd nst)))
+                              (fst nst) }}))).
 
   (** * FIXME: need to know children indices from [trs] are sound. *)
   Definition rqDownDownRule (oidx: IdxT)
-             (prec: OPrec)
-             (trs: OState -> Msg -> option (list IdxT * Msg)): Rule :=
+             (prec: OState -> list (Id Msg) -> Prop)
+             (trs: OState -> Msg -> list IdxT * Miv): Rule :=
     rule[ridx]
     :requires (MsgsFrom [downTo oidx] /\ MsgIdsFrom [msgId] /\
-               RqAccepting /\ DownLockFree /\ prec)
+               RqAccepting /\ DownLockFree /\
+               fun ost _ mins => prec ost mins)
     :transition
        (do (st -->
                (msg <-- getFirstMsg st.(msgs);
-                  nst <-- trs st.(ost) msg;
+                  nst ::= trs st.(ost) msg;
                 return {{ st.(ost),
                           addRq st.(orq) downRq msg
                                          (map rsUpFrom (fst nst)) (rsUpFrom oidx),
-                          map (fun cidx => (downTo cidx, snd nst)) (fst nst) }}))).
+                          map (fun cidx => (downTo cidx, rqMsg (snd nst)))
+                              (fst nst) }}))).
 
   Definition rsDownDownRule (rqId: IdxT)
              (prec: OPrec)
@@ -99,7 +127,7 @@ Section Template.
                    Msg (* an incoming message *) ->
                    Msg (* the original request *) ->
                    IdxT (* response back to *) ->
-                   option (OState * Msg)) :=
+                   OState * Miv) :=
     rule[ridx]
     :requires (MsgsFromORq upRq /\ MsgIdsFrom [msgId] /\ UpLockMsgId MRq rqId /\
                RsAccepting /\ DownLockFree /\ prec)
@@ -107,17 +135,17 @@ Section Template.
        (do (st --> (msg <-- getFirstMsg st.(msgs);
                       rq <-- getUpLockMsg st.(orq);
                       rsbTo <-- getUpLockIdxBack st.(orq);
-                      nst <-- trs st.(ost) msg rq rsbTo;
+                      nst ::= trs st.(ost) msg rq rsbTo;
                     return {{ fst nst,
                               removeRq st.(orq) upRq,
-                              [(rsbTo, snd nst)] }}))).
+                              [(rsbTo, rsMsg (snd nst))] }}))).
 
   Definition rsDownDownRuleS (rqId: IdxT)
              (prec: OPrec)
              (trs: OState ->
                    Msg (* an incoming message *) ->
                    Msg (* the original request *) ->
-                   option OState) :=
+                   OState) :=
     rule[ridx]
     :requires (MsgsFromORq upRq /\ MsgIdsFrom [msgId] /\ UpLockMsgId MRq rqId /\
                RsAccepting /\ DownLockFree /\ prec)
@@ -125,7 +153,7 @@ Section Template.
        (do (st --> (msg <-- getFirstMsg st.(msgs);
                       rq <-- getUpLockMsg st.(orq);
                       rsbTo <-- getUpLockIdxBack st.(orq);
-                      nst <-- trs st.(ost) msg rq;
+                      nst ::= trs st.(ost) msg rq;
                     return {{ nst, removeRq st.(orq) upRq, nil }}))).
 
   Definition rsUpDownRule (rqId: IdxT)
@@ -135,7 +163,7 @@ Section Template.
                    Msg (* the original request *) ->
                    list IdxT (* responses from *) ->
                    IdxT (* response back to *) ->
-                   option (OState * Msg)) :=
+                   OState * Miv) :=
     rule[ridx]
     :requires (MsgsFromORq downRq /\ MsgIdFromEach msgId /\
                DownLockMsgId MRq rqId /\ RsAccepting /\ prec)
@@ -143,10 +171,10 @@ Section Template.
        (do (st --> (rq <-- getDownLockMsg st.(orq);
                       rssFrom <-- getDownLockIndsFrom st.(orq);
                       rsbTo <-- getDownLockIdxBack st.(orq);
-                      nst <-- trs st.(ost) st.(msgs) rq rssFrom rsbTo;
+                      nst ::= trs st.(ost) st.(msgs) rq rssFrom rsbTo;
                     return {{ fst nst,
                               removeRq st.(orq) downRq,
-                              [(rsbTo, snd nst)] }}))).
+                              [(rsbTo, rsMsg (snd nst))] }}))).
 
   Definition rsUpUpRule (rqId: IdxT)
              (prec: OPrec)
@@ -155,7 +183,7 @@ Section Template.
                    Msg (* the original request *) ->
                    list IdxT (* responses from *) ->
                    IdxT (* response back to *) ->
-                   option (OState * Msg)) :=
+                   OState * Miv) :=
     rule[ridx]
     :requires (MsgsFromORq downRq /\ MsgIdFromEach msgId /\
                DownLockMsgId MRq rqId /\ RsAccepting /\ prec)
@@ -163,15 +191,15 @@ Section Template.
        (do (st --> (rq <-- getDownLockMsg st.(orq);
                       rssFrom <-- getDownLockIndsFrom st.(orq);
                       rsbTo <-- getDownLockIdxBack st.(orq);
-                      nst <-- trs st.(ost) st.(msgs) rq rssFrom rsbTo;
+                      nst ::= trs st.(ost) st.(msgs) rq rssFrom rsbTo;
                     return {{ fst nst,
                               removeRq st.(orq) downRq,
-                              [(rsbTo, snd nst)] }}))).
+                              [(rsbTo, rsMsg (snd nst))] }}))).
 
   (** * FIXME: need to know children indices from [trs] are sound. *)
-  Definition rsDownRqDownRule (rqId: IdxT)
+  Definition rsDownRqDownRule (oidx: IdxT) (rqId: IdxT)
              (prec: OPrec)
-             (trs: OState -> Msg -> option (list IdxT * Msg)) :=
+             (trs: OState -> Msg -> list IdxT * Miv) :=
     rule[ridx]
     :requires (MsgsFromORq upRq /\ MsgIdsFrom [msgId] /\
                UpLockMsgId MRq rqId /\
@@ -179,11 +207,11 @@ Section Template.
     :transition
        (do (st --> (rq <-- getUpLockMsg st.(orq);
                       rsbTo <-- getUpLockIdxBack st.(orq);
-                      nst <-- trs st.(ost) rq;
+                      nst ::= trs st.(ost) rq;
                     return {{ st.(ost),
                               addRq (removeRq st.(orq) upRq)
                                     downRq rq (map rsUpFrom (fst nst)) rsbTo,
-                              map (fun cidx => (downTo cidx, snd nst))
+                              map (fun cidx => (downTo cidx, rqMsg (snd nst)))
                                   (fst nst) }}))).
   
 End Template.
@@ -211,18 +239,141 @@ Notation "'rule.rsud' '[' RIDX ']' ':accepts' MSGID ':holding' RQID ':requires' 
 Notation "'rule.rsuu' '[' RIDX ']' ':accepts' MSGID ':holding' RQID ':requires' PREC ':transition' TRS" :=
   (rsUpUpRule RIDX MSGID RQID PREC%prec TRS%trs) (at level 5).
 
-Notation "'rule.rsrq' '[' RIDX ']' ':accepts' MSGID ':holding' RQID ':requires' PREC ':transition' TRS" :=
-  (rsDownRqDownRule RIDX MSGID RQID PREC%prec TRS%trs) (at level 5).
+Notation "'rule.rsrq' '[' RIDX ']' ':accepts' MSGID ':holding' RQID ':me' ME ':requires' PREC ':transition' TRS" :=
+  (rsDownRqDownRule RIDX MSGID ME RQID PREC%prec TRS%trs) (at level 5).
+
+Hint Unfold rqMsg rsMsg: RuleConds.
 
 Section Facts.
   Variable (dtr: DTree).
+  Hypothesis (Hdtr: TreeTopo dtr).
   Context `{oifc: OStateIfc}.
 
-  (* Lemma immDownRule_ImmDownRule: *)
-  (*   forall oidx ridx msgId cidx prec trs, *)
-  (*     parentIdxOf dtr cidx = Some oidx -> *)
-  (*     ImmDownRule dtr oidx (immDownRule ridx msgId cidx prec trs). *)
-  (* Proof. *)
+  Ltac solve_conds_ok :=
+    repeat red; cbn; unfold OPrecAnd, OPrecImp; intros;
+    disc_rule_conds_ex; try assumption.
+
+  Lemma immDownRule_ImmDownRule:
+    forall oidx ridx msgId cidx prec trs,
+      parentIdxOf dtr cidx = Some oidx ->
+      ImmDownRule dtr oidx (immDownRule ridx msgId cidx prec trs).
+  Proof.
+    unfold immDownRule; intros; repeat split;
+      try solve_rule_conds_ex.
+    - apply Hdtr in H; dest; assumption.
+    - apply Hdtr in H; dest; assumption.
+  Qed.
+
+  Lemma immUpRule_ImmUpRule:
+    forall oidx ridx msgId cidx prec trs,
+      parentIdxOf dtr cidx = Some oidx ->
+      ImmUpRule dtr cidx (immUpRule ridx msgId cidx prec trs).
+  Proof.
+    unfold immUpRule; intros; repeat split;
+      try solve_rule_conds_ex.
+    - apply Hdtr in H; dest; assumption.
+    - apply Hdtr in H; dest; assumption.
+  Qed.
+
+  Lemma rqUpUpRule_RqFwdRule:
+    forall sys oidx pidx ridx msgId cidx prec trs,
+      parentIdxOf dtr cidx = Some oidx ->
+      parentIdxOf dtr oidx = Some pidx ->
+      RqFwdRule dtr sys oidx (rqUpUpRule ridx msgId cidx oidx prec trs).
+  Proof.
+    unfold rqUpUpRule; intros; split.
+    - repeat split; solve_rule_conds_ex.
+      destruct (idm <-- hd_error mins; Some (valOf idm))%trs;
+        reflexivity.
+    - left; repeat split; solve_rule_conds_ex.
+      + apply Hdtr in H; dest; assumption.
+      + apply Hdtr in H0; dest; assumption.
+      + apply Hdtr in H0; dest; assumption.
+      + apply Hdtr in H; dest; assumption.
+  Qed.
+
+  Lemma rqUpDownRule_RqFwdRule:
+    forall sys oidx ridx msgId cidx prec trs,
+      parentIdxOf dtr cidx = Some oidx ->
+      RqFwdRule dtr sys oidx (rqUpDownRule ridx msgId cidx oidx prec trs).
+  Proof.
+    unfold rqUpDownRule; intros; split.
+    - repeat split; solve_rule_conds_ex.
+      + apply Forall_forall; intros msg ?.
+        apply in_map_iff in H0.
+        destruct H0 as [midx ?]; dest; subst; reflexivity.
+      + destruct (idm <-- hd_error mins; Some (valOf idm))%trs;
+          reflexivity.
+    - right; left; repeat red; repeat ssplit.
+      + solve_rule_conds_ex.
+      + solve_rule_conds_ex.
+      + solve_rule_conds_ex.
+        admit. (** TODO: [DownLockFreeSuff] is too strong. *)
+      + solve_rule_conds_ex.
+        all: admit. (** TODO: existence of [upCObj] & valid children *)
+  Admitted.
+
+  Lemma rqDownDownRule_RqFwdRule:
+    forall sys oidx ridx msgId prec trs,
+      RqFwdRule dtr sys oidx (rqDownDownRule ridx msgId oidx prec trs).
+  Proof.
+    unfold rqDownDownRule; intros; split.
+    - repeat split; solve_rule_conds_ex.
+      + apply Forall_forall; intros msg ?.
+        apply in_map_iff in H.
+        destruct H as [midx ?]; dest; subst; reflexivity.
+      + destruct (idm <-- hd_error mins; Some (valOf idm))%trs;
+          reflexivity.
+    - right; left; repeat red; repeat ssplit.
+      + solve_rule_conds_ex.
+      + solve_rule_conds_ex.
+      + solve_rule_conds_ex.
+      + solve_rule_conds_ex.
+        all: admit. (** TODO: existence of [upCObj] & valid children *)
+  Admitted.
+
+  Lemma rsDownDownRule_RsBackRule:
+    forall ridx msgId rqId prec trs,
+      RsBackRule (rsDownDownRule ridx msgId rqId prec trs).
+  Proof.
+    unfold rsDownDownRule; intros; split.
+    - left; repeat red; repeat ssplit; solve_rule_conds_ex.
+    - repeat red; repeat ssplit; solve_rule_conds_ex.
+  Qed.
+
+  Lemma rsUpDownRule_RsBackRule:
+    forall ridx msgId rqId prec trs,
+      RsBackRule (rsUpDownRule ridx msgId rqId prec trs).
+  Proof.
+    unfold rsUpDownRule; intros; split.
+    - right; repeat red; repeat ssplit; solve_rule_conds_ex.
+    - repeat red; repeat ssplit; solve_rule_conds_ex.
+  Qed.
+  
+  Lemma rsUpUpRule_RsBackRule:
+    forall ridx msgId rqId prec trs,
+      RsBackRule (rsUpUpRule ridx msgId rqId prec trs).
+  Proof.
+    unfold rsUpUpRule; intros; split.
+    - right; repeat red; repeat ssplit; solve_rule_conds_ex.
+    - repeat red; repeat ssplit; solve_rule_conds_ex.
+  Qed.
+
+  Lemma rsDownRqDownRule_RsDownRqDownRule:
+    forall sys oidx ridx msgId rqId prec trs,
+      RsDownRqDownRule dtr sys oidx (rsDownRqDownRule ridx msgId oidx rqId prec trs).
+  Proof.
+    unfold rsDownRqDownRule; intros; red; repeat ssplit.
+    - solve_rule_conds_ex.
+    - solve_rule_conds_ex.
+    - solve_rule_conds_ex.
+      apply Forall_forall; intros msg ?.
+      apply in_map_iff in H1.
+      destruct H1 as [midx ?]; dest; subst; reflexivity.
+    - solve_rule_conds_ex.
+    - solve_rule_conds_ex.
+      all: admit. (** TODO: existence of [upCObj] & valid children *)
+  Admitted.
 
 End Facts.
 
