src/Ex/MsiSv/MsiSvInv.v
@@ -1414,7 +1414,7 @@ Section Inv.
 
         split.
         + pose proof H3.
-          eapply atomic_rsDown_singleton with (oidx:= child1Idx) in H24;
+          eapply atomic_rsDown_singleton with (oidx:= child1Idx) in H22;
             try exact H; eauto; [|red; auto].
           subst; rewrite removeOnce_nil; simpl.
           repeat constructor.
@@ -1423,8 +1423,8 @@ Section Inv.
           intuition idtac; try solve_msi_false; try solve_msi.
           * apply invalidMsgs_other_msg_id_enqMP; [|solve_not_in].
             apply invalidMsgs_deqMP; assumption.
-          * apply msgExistsSig_enqMP_or in H36; destruct H36; [discriminate|].
-            apply msgExistsSig_deqMP_inv in H36; auto.
+          * apply msgExistsSig_enqMP_or in H35; destruct H35; [discriminate|].
+            apply msgExistsSig_deqMP_inv in H35; auto.
           * apply childInvalid_enqMP.
             apply childInvalid_other_midx_deqMP; [|discriminate].
             assumption.
@@ -1474,7 +1474,7 @@ Section Inv.
 
         split.
         + pose proof H3.
-          eapply atomic_rsDown_singleton with (oidx:= child1Idx) in H24;
+          eapply atomic_rsDown_singleton with (oidx:= child1Idx) in H22;
             try exact H; eauto; [|red; auto].
           subst; rewrite removeOnce_nil; simpl.
           repeat constructor.
@@ -1488,11 +1488,11 @@ Section Inv.
               try exact Hr1; try reflexivity; try eassumption.
             { simpl; tauto. }
             { apply FirstMP_InMP; assumption. }
-            { rewrite H15; discriminate. }
+            { rewrite H14; discriminate. }
           * apply invalidMsgs_other_midx_enqMP; [|solve_not_in].
             apply invalidMsgs_deqMP; assumption.
-          * apply msgExistsSig_enqMP_or in H37; destruct H37; [discriminate|].
-            apply msgExistsSig_deqMP_inv in H37; auto.
+          * apply msgExistsSig_enqMP_or in H36; destruct H36; [discriminate|].
+            apply msgExistsSig_deqMP_inv in H36; auto.
           * apply childInvalid_enqMP.
             apply childInvalid_other_midx_deqMP; [|discriminate].
             assumption.
@@ -1579,7 +1579,7 @@ Section Inv.
 
         split.
         + pose proof H3.
-          eapply atomic_rsDown_singleton with (oidx:= child2Idx) in H24;
+          eapply atomic_rsDown_singleton with (oidx:= child2Idx) in H22;
             try exact H; eauto; [|red; auto].
           subst; rewrite removeOnce_nil; simpl.
           repeat constructor.
@@ -1588,8 +1588,8 @@ Section Inv.
           intuition idtac; try solve_msi_false; try solve_msi.
           * apply invalidMsgs_other_msg_id_enqMP; [|solve_not_in].
             apply invalidMsgs_deqMP; assumption.
-          * apply msgExistsSig_enqMP_or in H36; destruct H36; [discriminate|].
-            apply msgExistsSig_deqMP_inv in H36; auto.
+          * apply msgExistsSig_enqMP_or in H35; destruct H35; [discriminate|].
+            apply msgExistsSig_deqMP_inv in H35; auto.
           * apply childInvalid_enqMP.
             apply childInvalid_other_midx_deqMP; [|discriminate].
             assumption.
@@ -1639,7 +1639,7 @@ Section Inv.
 
         split.
         + pose proof H3.
-          eapply atomic_rsDown_singleton with (oidx:= child2Idx) in H24;
+          eapply atomic_rsDown_singleton with (oidx:= child2Idx) in H22;
             try exact H; eauto; [|red; auto].
           subst; rewrite removeOnce_nil; simpl.
           repeat constructor.
@@ -1648,8 +1648,8 @@ Section Inv.
           intuition idtac; try solve_msi_false; try solve_msi.
           * apply invalidMsgs_other_midx_enqMP; [|solve_not_in].
             apply invalidMsgs_deqMP; assumption.
-          * apply msgExistsSig_enqMP_or in H37; destruct H37; [discriminate|].
-            apply msgExistsSig_deqMP_inv in H37; auto.
+          * apply msgExistsSig_enqMP_or in H36; destruct H36; [discriminate|].
+            apply msgExistsSig_deqMP_inv in H36; auto.
           * apply invalidMsgs_other_midx_enqMP; [|solve_not_in].
             apply invalidMsgs_deqMP.
             eapply invalidMsgs_if_rsDown_exists
@@ -1657,7 +1657,7 @@ Section Inv.
               try exact Hr1; try reflexivity; try eassumption.
             { simpl; tauto. }
             { apply FirstMP_InMP; assumption. }
-            { rewrite H15; discriminate. }
+            { rewrite H14; discriminate. }
           * apply childInvalid_enqMP.
             apply childInvalid_other_midx_deqMP; [|discriminate].
             assumption.
@@ -1875,49 +1875,6 @@ Section Inv.
           get_child_uplock_from_parent.
           eauto.
         }
-        destruct H34 as [corq1 [? ?]].
-
-        split.
-        + good_footprint_get parentIdx.
-          disc_rule_conds.
-          apply Forall_app.
-          * simpl.
-            red in H5; simpl in H5.
-            rewrite <-H7 in H42.
-            eapply atomic_rsUps_preserves_msg_out_preds
-              with (rsUps:= [(c2pRs, rmsg)]) in H5;
-              try exact H9; try eassumption; eauto.
-            { right; right; left; reflexivity. }
-            { reflexivity. }
-            { repeat constructor; intro Hx; elim Hx. }
-            { apply SubList_cons; [assumption|].
-              apply SubList_nil.
-            }
-          * repeat constructor.
-            red; simpl.
-            solve_rule_conds_ex.
-            
-        + red in H6; red.
-          disc_rule_conds_ex.
-          intuition idtac; try solve_msi_false; try discriminate.
-          * clear -H12; solve_msi.
-          * clear -H12; solve_msi.
-            
-      - (** [parentGetDownRsI] *)
-        disc_rule_conds_ex.
-        disc_msg_preds H4.
-        disc_rule_conds_ex.
-        red in Hibinv.
-        disc_rule_conds_ex.
-
-        assert (exists corq1,
-                   orqs@[child1Idx] = Some corq1 /\
-                   corq1@[upRq] <> None).
-        { clear Hnulinv Hpdlinv Hndlinv.
-          get_lock_inv (child child1Idx ec1 ce1 c1pRq c1pRs pc1) impl.
-          get_child_uplock_from_parent.
-          eauto.
-        }
         destruct H33 as [corq1 [? ?]].
 
         split.
@@ -1939,15 +1896,58 @@ Section Inv.
           * repeat constructor.
             red; simpl.
             solve_rule_conds_ex.
+            
         + red in H6; red.
           disc_rule_conds_ex.
           intuition idtac; try solve_msi_false; try discriminate.
-          * clear -H12; solve_msi.
-          * clear -H12; solve_msi.
+          * clear -H11; solve_msi.
+          * clear -H11; solve_msi.
+            
+      - (** [parentGetDownRsI] *)
+        disc_rule_conds_ex.
+        disc_msg_preds H4.
+        disc_rule_conds_ex.
+        red in Hibinv.
+        disc_rule_conds_ex.
+
+        assert (exists corq1,
+                   orqs@[child1Idx] = Some corq1 /\
+                   corq1@[upRq] <> None).
+        { clear Hnulinv Hpdlinv Hndlinv.
+          get_lock_inv (child child1Idx ec1 ce1 c1pRq c1pRs pc1) impl.
+          get_child_uplock_from_parent.
+          eauto.
+        }
+        destruct H32 as [corq1 [? ?]].
+
+        split.
+        + good_footprint_get parentIdx.
+          disc_rule_conds.
+          apply Forall_app.
+          * simpl.
+            red in H5; simpl in H5.
+            rewrite <-H7 in H40.
+            eapply atomic_rsUps_preserves_msg_out_preds
+              with (rsUps:= [(c2pRs, rmsg)]) in H5;
+              try exact H9; try eassumption; eauto.
+            { right; right; left; reflexivity. }
+            { reflexivity. }
+            { repeat constructor; intro Hx; elim Hx. }
+            { apply SubList_cons; [assumption|].
+              apply SubList_nil.
+            }
+          * repeat constructor.
+            red; simpl.
+            solve_rule_conds_ex.
+        + red in H6; red.
+          disc_rule_conds_ex.
+          intuition idtac; try solve_msi_false; try discriminate.
+          * clear -H11; solve_msi.
+          * clear -H11; solve_msi.
           * exfalso.
             clear Hpulinv Hpdlinv Hndlinv.
             get_lock_inv (child child1Idx ec1 ce1 c1pRq c1pRs pc1) impl.
-            destruct H46 as [[midx msg] ?]; dest; inv H47.
+            destruct H45 as [[midx msg] ?]; dest; inv H46.
             exfalso_uplock_rq_rs parentIdx c1pRq pc1.
           * left; assumption.
           * clear Hnulinv Hndlinv.
@@ -2079,7 +2079,7 @@ Section Inv.
 
         split.
         + pose proof H3.
-          eapply atomic_rqUp_singleton with (oidx:= child1Idx) in H30;
+          eapply atomic_rqUp_singleton with (oidx:= child1Idx) in H29;
             try exact H; eauto; [|red; auto].
           subst; rewrite removeOnce_nil; simpl.
           repeat constructor.
@@ -2090,7 +2090,7 @@ Section Inv.
           intuition idtac; try solve_msi_false.
           * apply invalidMsgs_other_midx_enqMP; [|solve_not_in].
             apply invalidMsgs_deqMP; assumption.
-          * exfalso; clear -H14 H44; solve_msi.
+          * exfalso; clear -H13 H43; solve_msi.
           * right; eexists (_, _); split.
             { apply InMP_or_enqMP; left; simpl; eauto. }
             { reflexivity. }
@@ -2251,51 +2251,6 @@ Section Inv.
           get_child_uplock_from_parent.
           eauto.
         }
-        destruct H34 as [corq2 [? ?]].
-
-        split.
-        + good_footprint_get parentIdx.
-          disc_rule_conds.
-          apply Forall_app.
-          * simpl.
-            red in H5; simpl in H5.
-            rewrite <-H7 in H42.
-            eapply atomic_rsUps_preserves_msg_out_preds
-              with (rsUps:= [(c1pRs, rmsg)]) in H5;
-              try exact H9; try eassumption; eauto.
-            { right; right; left; reflexivity. }
-            { reflexivity. }
-            { repeat constructor; intro Hx; elim Hx. }
-            { apply SubList_cons; [assumption|].
-              apply SubList_nil.
-            }
-          * repeat constructor.
-            red; simpl.
-            solve_rule_conds_ex.
-            
-        + red in H6; red.
-          disc_rule_conds_ex.
-          intuition idtac; try solve_msi_false; try discriminate.
-          * clear -H12; solve_msi.
-          * clear -H12; solve_msi.
-            
-      - (** [parentGetDownRsI] *)
-        disc_rule_conds_ex.
-
-        disc_msg_preds H4.
-        disc_rule_conds_ex.
-
-        red in Hibinv.
-        disc_rule_conds_ex.
-
-        assert (exists corq2,
-                   orqs@[child2Idx] = Some corq2 /\
-                   corq2@[upRq] <> None).
-        { clear Hnulinv Hpdlinv Hndlinv.
-          get_lock_inv (child child2Idx ec2 ce2 c2pRq c2pRs pc2) impl.
-          get_child_uplock_from_parent.
-          eauto.
-        }
         destruct H33 as [corq2 [? ?]].
 
         split.
@@ -2317,15 +2272,60 @@ Section Inv.
           * repeat constructor.
             red; simpl.
             solve_rule_conds_ex.
+            
         + red in H6; red.
           disc_rule_conds_ex.
           intuition idtac; try solve_msi_false; try discriminate.
-          * clear -H12; solve_msi.
-          * clear -H12; solve_msi.
+          * clear -H11; solve_msi.
+          * clear -H11; solve_msi.
+            
+      - (** [parentGetDownRsI] *)
+        disc_rule_conds_ex.
+
+        disc_msg_preds H4.
+        disc_rule_conds_ex.
+
+        red in Hibinv.
+        disc_rule_conds_ex.
+
+        assert (exists corq2,
+                   orqs@[child2Idx] = Some corq2 /\
+                   corq2@[upRq] <> None).
+        { clear Hnulinv Hpdlinv Hndlinv.
+          get_lock_inv (child child2Idx ec2 ce2 c2pRq c2pRs pc2) impl.
+          get_child_uplock_from_parent.
+          eauto.
+        }
+        destruct H32 as [corq2 [? ?]].
+
+        split.
+        + good_footprint_get parentIdx.
+          disc_rule_conds.
+          apply Forall_app.
+          * simpl.
+            red in H5; simpl in H5.
+            rewrite <-H7 in H40.
+            eapply atomic_rsUps_preserves_msg_out_preds
+              with (rsUps:= [(c1pRs, rmsg)]) in H5;
+              try exact H9; try eassumption; eauto.
+            { right; right; left; reflexivity. }
+            { reflexivity. }
+            { repeat constructor; intro Hx; elim Hx. }
+            { apply SubList_cons; [assumption|].
+              apply SubList_nil.
+            }
+          * repeat constructor.
+            red; simpl.
+            solve_rule_conds_ex.
+        + red in H6; red.
+          disc_rule_conds_ex.
+          intuition idtac; try solve_msi_false; try discriminate.
+          * clear -H11; solve_msi.
+          * clear -H11; solve_msi.
           * exfalso.
             clear Hpulinv Hpdlinv Hndlinv.
             get_lock_inv (child child2Idx ec2 ce2 c2pRq c2pRs pc2) impl.
-            destruct H46 as [[midx msg] ?]; dest; inv H47.
+            destruct H45 as [[midx msg] ?]; dest; inv H46.
             exfalso_uplock_rq_rs parentIdx c2pRq pc2.
           * left; assumption.
           * clear Hnulinv Hndlinv.
@@ -2457,7 +2457,7 @@ Section Inv.
 
         split.
         + pose proof H3.
-          eapply atomic_rqUp_singleton with (oidx:= child2Idx) in H30;
+          eapply atomic_rqUp_singleton with (oidx:= child2Idx) in H29;
             try exact H; eauto; [|red; auto].
           subst; rewrite removeOnce_nil; simpl.
           repeat constructor.
@@ -2468,7 +2468,7 @@ Section Inv.
           intuition idtac; try solve_msi_false.
           * apply invalidMsgs_other_midx_enqMP; [|solve_not_in].
             apply invalidMsgs_deqMP; assumption.
-          * exfalso; clear -H14 H44; solve_msi.
+          * exfalso; clear -H13 H43; solve_msi.
           * apply childInvalid_enqMP.
             apply childInvalid_other_midx_deqMP; [|discriminate].
             assumption.
