src/Ex/MsiSv/MsiSvSim.v
@@ -35,10 +35,10 @@ Section Sim.
 
     Definition DirMsgCoh (idm: Id Msg) :=
       match case (sigOf idm) on sig_dec default True with
-      | (pc, (MRs, msiRsS)): (valOf idm).(msg_value) = VNat cv
-      | (cpRs, (MRs, msiDownRsS)): (valOf idm).(msg_value) = VNat cv
+      | (pc, (MRs, msiRsS)): (valOf idm).(msg_value) = cv
+      | (cpRs, (MRs, msiDownRsS)): (valOf idm).(msg_value) = cv
       | (cpRq, (MRq, msiRqI)):
-          (msiS <= cost#[implStatusIdx] -> (valOf idm).(msg_value) = VNat cv)
+          (msiS <= cost#[implStatusIdx] -> (valOf idm).(msg_value) = cv)
       end.
     
     Definition DirMsgsCoh :=
@@ -910,9 +910,9 @@ Section Sim.
         get_lock_inv (child child1Idx ec1 ce1 c1pRq c1pRs pc1) impl.
         disc_rule_conds_const.
 
-        assert (n = fst sost)
-          by (disc_DirMsgsCoh_by_FirstMP H15 H55; congruence).
-        subst.
+        assert (msg_value rmsg = fst sost)
+          by (disc_DirMsgsCoh_by_FirstMP H15 H54; assumption).
+        rewrite H17 in *.
 
         red; simpl; split.
         + eapply SimStateIntro with (cv:= fst sost).
@@ -959,19 +959,18 @@ Section Sim.
         disc_rule_conds_ex.
         spec_case_set 0 ec1.
 
-        rewrite H21 in H1.
+        rewrite H20 in H1.
         disc_rule_conds_ex.
               
         red; simpl; split.
-        + eapply SimStateIntro with (cv:= n).
-          * rewrite Hmsg.
-            solve_rule_conds_ex.
+        + eapply SimStateIntro with (cv:= msg_value rmsg).
+          * solve_rule_conds_ex.
           * red; simpl.
             disc_rule_conds_ex.
             intuition idtac; try solve_msi_false.
             apply invalidMsgs_DirMsgsCoh.
-            apply H30; auto.
-            clear -H21; solve_msi.
+            apply H29; auto.
+            clear -H20; solve_msi.
         + solve_sim_ext_mp.
 
       - (** [childSetRqM] *)
@@ -1006,16 +1005,15 @@ Section Sim.
         disc_rule_conds_ex.
 
         red; simpl; split.
-        + eapply SimStateIntro with (cv:= n).
-          * rewrite Hmsg.
-            solve_rule_conds_ex.
+        + eapply SimStateIntro with (cv:= msg_value (rqi_msg rqi)).
+          * solve_rule_conds_ex.
           * red; simpl.
             disc_rule_conds_ex.
             intuition idtac.
             { solve_msi_false. }
             { apply invalidMsgs_DirMsgsCoh.
-              rewrite <-H62 in H29.
-              apply H29; auto.
+              rewrite <-H61 in H28.
+              apply H28; auto.
             }
             { solve_msi_false. }
             { apply DirMsgsCoh_other_msg_id_enqMP; [|solve_not_in].
@@ -1154,9 +1152,9 @@ Section Sim.
         get_lock_inv (child child2Idx ec2 ce2 c2pRq c2pRs pc2) impl.
         disc_rule_conds_const.
 
-        assert (n = fst sost)
-          by (disc_DirMsgsCoh_by_FirstMP H16 H55; congruence).
-        subst.
+        assert (msg_value rmsg = fst sost)
+          by (disc_DirMsgsCoh_by_FirstMP H16 H54; congruence).
+        rewrite H17 in *.
 
         red; simpl; split.
         + eapply SimStateIntro with (cv:= fst sost).
@@ -1203,19 +1201,18 @@ Section Sim.
         disc_rule_conds_ex.
         spec_case_set 1 ec2.
 
-        rewrite H21 in H53.
+        rewrite H20 in H52.
         disc_rule_conds_ex.
               
         red; simpl; split.
-        + eapply SimStateIntro with (cv:= n).
-          * rewrite Hmsg.
-            solve_rule_conds_ex.
+        + eapply SimStateIntro with (cv:= msg_value rmsg).
+          * solve_rule_conds_ex.
           * red; simpl.
             disc_rule_conds_ex.
             intuition idtac; try solve_msi_false.
             apply invalidMsgs_DirMsgsCoh.
-            apply H31; auto.
-            clear -H21; solve_msi.
+            apply H30; auto.
+            clear -H20; solve_msi.
         + solve_sim_ext_mp.
 
       - (** [childSetRqM] *)
@@ -1250,9 +1247,8 @@ Section Sim.
         disc_rule_conds_ex.
 
         red; simpl; split.
-        + eapply SimStateIntro with (cv:= n).
-          * rewrite Hmsg.
-            solve_rule_conds_ex.
+        + eapply SimStateIntro with (cv:= msg_value (rqi_msg rqi)).
+          * solve_rule_conds_ex.
           * red; simpl.
             disc_rule_conds_ex.
             intuition idtac.
@@ -1263,8 +1259,8 @@ Section Sim.
               apply invalidMsgs_DirMsgsCoh; assumption.
             }
             { apply invalidMsgs_DirMsgsCoh.
-              rewrite <-H62 in H30.
-              apply H30; auto.
+              rewrite <-H61 in H29.
+              apply H29; auto.
             }
         + solve_sim_ext_mp.
 
@@ -1361,7 +1357,7 @@ Section Sim.
                     parentIdx pc1 msg
                     {| msg_id:= msiRsS;
                        msg_type:= MRs;
-                       msg_value:= VNat (fst post) |}.
+                       msg_value:= fst post |}.
                 }
               }
               { apply DirMsgsCoh_enqMP.
@@ -1403,7 +1399,7 @@ Section Sim.
                       parentIdx pc1 msg
                       {| msg_id:= msiRsS;
                          msg_type:= MRs;
-                         msg_value:= VNat (fst post) |}.
+                         msg_value:= fst post |}.
                   }
                 }
                 { apply DirMsgsCoh_enqMP.
@@ -1471,7 +1467,7 @@ Section Sim.
                     parentIdx pc1 msg
                     {| msg_id:= msiRsM;
                        msg_type:= MRs;
-                       msg_value:= VUnit |}.
+                       msg_value:= O |}.
                 }
               }
               { apply DirMsgsCoh_other_msg_id_enqMP; [|solve_not_in].
@@ -1506,18 +1502,18 @@ Section Sim.
         disc_rule_conds_ex.
         spec_case_silent.
 
-        inv H60.
+        inv H59.
         unfold setDir in *; simpl in *.
 
         (* Discharge the downlock invariant *)
-        specialize (H37 eq_refl); dest.
+        specialize (H36 eq_refl); dest.
         disc_rule_conds_ex.
 
         (* To get [DirMsgsCoh (fst sost) cost2 ..]  *)
-        specialize (H16 ltac:(clear -H43; solve_msi)); dest.
-        pose proof H60.
-        disc_DirMsgsCoh_by_FirstMP H61 H54.
-        rewrite Hmsg in H61; inv H61.
+        specialize (H16 ltac:(clear -H42; solve_msi)); dest.
+        pose proof H59.
+        disc_DirMsgsCoh_by_FirstMP H60 H53.
+        rewrite H60 in *.
 
         red; simpl; split.
         + eapply SimStateIntro with (cv:= fst sost).
@@ -1525,9 +1521,9 @@ Section Sim.
           * red; simpl.
             disc_rule_conds_ex.
             intuition idtac.
-            { destruct H47.
+            { destruct H46.
               { exfalso; simpl in *; solve_msi_false. }
-              { destruct H47 as [[midx msg] [? ?]]; inv H65.
+              { destruct H46 as [[midx msg] [? ?]]; inv H65.
                 clear Hpulinv.
                 get_lock_inv (child child1Idx ec1 ce1 c1pRq c1pRs pc1) impl.
                 disc_rule_conds_const.
@@ -1536,7 +1532,7 @@ Section Sim.
                   parentIdx pc1 msg
                   {| msg_id:= msiRsS;
                      msg_type:= MRs;
-                     msg_value:= VNat (fst sost) |}.
+                     msg_value:= fst sost |}.
               }
             }
             { apply DirMsgsCoh_enqMP.
@@ -1554,10 +1550,10 @@ Section Sim.
         disc_rule_conds_ex.
         spec_case_silent.
 
-        inv H61.
+        inv H60.
         unfold setDir in *; simpl in *.
 
-        specialize (H57 eq_refl).
+        specialize (H56 eq_refl).
         disc_rule_conds_ex.
 
         red; simpl; split.
@@ -1574,9 +1570,9 @@ Section Sim.
             { assert (fst (fst (snd (snd post))) = msiI) by (clear -g; solve_msi).
               disc_rule_conds_ex.
               intuition idtac; try solve_msi_false.
-              { destruct H47.
+              { destruct H46.
                 { exfalso; simpl in *; solve_msi_false. }
-                { destruct H47 as [[midx msg] [? ?]]; inv H66.
+                { destruct H46 as [[midx msg] [? ?]]; inv H65.
                   clear Hpulinv.
                   get_lock_inv (child child1Idx ec1 ce1 c1pRq c1pRs pc1) impl.
                   disc_rule_conds_const.
@@ -1585,7 +1581,7 @@ Section Sim.
                     parentIdx pc1 msg
                     {| msg_id:= msiRsM;
                        msg_type:= MRs;
-                       msg_value:= VUnit |}.
+                       msg_value:= O |}.
                 }
               }
               { apply DirMsgsCoh_other_msg_id_enqMP; [|solve_not_in].
@@ -1659,16 +1655,16 @@ Section Sim.
         unfold getDir in *; simpl in *.
 
         (* discharging [ImplStateInv] *)
-        assert (n = fst sost).
-        { specialize (H15 ltac:(clear -H21; solve_msi)); dest.
-          disc_DirMsgsCoh_by_FirstMP H15 H57.
+        assert (msg_value rmsg = fst sost).
+        { specialize (H15 ltac:(clear -H20; solve_msi)); dest.
+          disc_DirMsgsCoh_by_FirstMP H15 H56.
           assert (msiM <= fst (snd cost1)).
-          { apply H52; auto.
-            { rewrite H21; auto. }
+          { apply H51; auto.
+            { rewrite H20; auto. }
             { exists (c1pRq, rmsg); split.
               { apply FirstMP_InMP; assumption. }
               { unfold sigOf; simpl.
-                rewrite H56, H9; reflexivity.
+                rewrite H55, H9; reflexivity.
               }
             }
           }
@@ -1715,7 +1711,7 @@ Section Sim.
                     parentIdx pc2 msg
                     {| msg_id:= msiRsS;
                        msg_type:= MRs;
-                       msg_value:= VNat (fst post) |}.
+                       msg_value:= fst post |}.
                 }
               }
               { apply DirMsgsCoh_enqMP.
@@ -1757,7 +1753,7 @@ Section Sim.
                       parentIdx pc2 msg
                       {| msg_id:= msiRsS;
                          msg_type:= MRs;
-                         msg_value:= VNat (fst post) |}.
+                         msg_value:= fst post |}.
                   }
                 }
                 { apply DirMsgsCoh_enqMP.
@@ -1822,7 +1818,7 @@ Section Sim.
                     parentIdx pc2 msg
                     {| msg_id:= msiRsM;
                        msg_type:= MRs;
-                       msg_value:= VUnit |}.
+                       msg_value:= O |}.
                 }
               }
               { apply DirMsgsCoh_other_msg_id_enqMP; [|solve_not_in].
@@ -1857,18 +1853,18 @@ Section Sim.
         disc_rule_conds_ex.
         spec_case_silent.
 
-        inv H60.
+        inv H59.
         unfold setDir in *; simpl in *.
 
         (* Discharge the downlock invariant *)
-        specialize (H24 eq_refl); dest.
+        specialize (H23 eq_refl); dest.
         disc_rule_conds_ex.
 
         (* To get [DirMsgsCoh (fst sost) cost1 ..]  *)
-        specialize (H15 ltac:(clear -H44; solve_msi)); dest.
-        pose proof H60.
-        disc_DirMsgsCoh_by_FirstMP H61 H54.
-        rewrite Hmsg in H61; inv H61.
+        specialize (H15 ltac:(clear -H43; solve_msi)); dest.
+        pose proof H59.
+        disc_DirMsgsCoh_by_FirstMP H60 H53.
+        rewrite H60 in *.
 
         red; simpl; split.
         + eapply SimStateIntro with (cv:= fst sost).
@@ -1879,9 +1875,9 @@ Section Sim.
             { apply DirMsgsCoh_other_midx_enqMP; [|solve_not_in].
               apply DirMsgsCoh_deqMP; assumption.
             }
-            { destruct H48.
+            { destruct H47.
               { exfalso; simpl in *; solve_msi_false. }
-              { destruct H48 as [[midx msg] [? ?]]; inv H65.
+              { destruct H47 as [[midx msg] [? ?]]; inv H65.
                 clear Hpulinv.
                 get_lock_inv (child child2Idx ec2 ce2 c2pRq c2pRs pc2) impl.
                 disc_rule_conds_const.
@@ -1890,7 +1886,7 @@ Section Sim.
                   parentIdx pc2 msg
                   {| msg_id:= msiRsS;
                      msg_type:= MRs;
-                     msg_value:= VNat (fst sost) |}.
+                     msg_value:= fst sost |}.
               }
             }
             { apply DirMsgsCoh_enqMP.
@@ -1905,10 +1901,10 @@ Section Sim.
         disc_rule_conds_ex.
         spec_case_silent.
 
-        inv H61.
+        inv H60.
         unfold setDir in *; simpl in *.
 
-        specialize (H37 eq_refl).
+        specialize (H36 eq_refl).
         disc_rule_conds_ex.
 
         red; simpl; split.
@@ -1925,9 +1921,9 @@ Section Sim.
             { assert (snd (fst (snd (snd post))) = msiI) by (clear -g; solve_msi).
               disc_rule_conds_ex.
               intuition idtac; try solve_msi_false.
-              { destruct H48.
+              { destruct H47.
                 { exfalso; simpl in *; solve_msi_false. }
-                { destruct H48 as [[midx msg] [? ?]]; inv H65.
+                { destruct H47 as [[midx msg] [? ?]]; inv H64.
                   clear Hpulinv.
                   get_lock_inv (child child2Idx ec2 ce2 c2pRq c2pRs pc2) impl.
                   disc_rule_conds_const.
@@ -1936,7 +1932,7 @@ Section Sim.
                     parentIdx pc2 msg
                     {| msg_id:= msiRsM;
                        msg_type:= MRs;
-                       msg_value:= VUnit |}.
+                       msg_value:= O |}.
                 }
               }
               { apply DirMsgsCoh_other_msg_id_enqMP; [|solve_not_in].
@@ -2010,16 +2006,16 @@ Section Sim.
         unfold getDir in *; simpl in *.
 
         (* discharging [ImplStateInv] *)
-        assert (n = fst sost).
-        { specialize (H16 ltac:(clear -H21; solve_msi)); dest.
-          disc_DirMsgsCoh_by_FirstMP H16 H57.
+        assert (msg_value rmsg = fst sost).
+        { specialize (H16 ltac:(clear -H20; solve_msi)); dest.
+          disc_DirMsgsCoh_by_FirstMP H16 H56.
           assert (msiM <= fst (snd cost2)).
-          { apply H51; auto.
-            { rewrite H21; auto. }
+          { apply H50; auto.
+            { rewrite H20; auto. }
             { exists (c2pRq, rmsg); split.
               { apply FirstMP_InMP; assumption. }
               { unfold sigOf; simpl.
-                rewrite H56, H9; reflexivity.
+                rewrite H55, H9; reflexivity.
               }
             }
           }
